Weidenbach_Book/IsaSAT/IsaSAT_Bump_Heuristics_Init_State.thy
@@ -1,0 +1,308 @@
+theory IsaSAT_Bump_Heuristics_Init_State
+imports Watched_Literals_VMTF 
+(*
+  IsaSAT_VSIDS
+  *)
+  Tuple4
+begin
+
+type_synonym vmtf_remove_int_option_fst_As = \<open>nat_vmtf_node list \<times> nat \<times> nat option \<times> nat option \<times> nat option\<close>
+
+
+definition isa_vmtf_init
+   :: \<open>nat multiset \<Rightarrow> (nat, nat) ann_lits \<Rightarrow> vmtf_remove_int_option_fst_As set\<close>
+where
+  \<open>isa_vmtf_init \<A>\<^sub>i\<^sub>n M = {(ns, m, fst_As, lst_As, next_search).
+   \<A>\<^sub>i\<^sub>n \<noteq> {#} \<longrightarrow> (fst_As \<noteq> None \<and> lst_As \<noteq> None \<and> (ns, m, the fst_As, the lst_As, next_search) \<in> vmtf \<A>\<^sub>i\<^sub>n M)}\<close>
+
+(*TODO: share the to_remove part of Bump_Heuristics_Init*)
+type_synonym bump_heuristics_init = \<open>(vmtf_remove_int_option_fst_As, vmtf_remove_int_option_fst_As, bool, nat list \<times> bool list) tuple4\<close>
+
+abbreviation Bump_Heuristics_Init :: \<open>_ \<Rightarrow> _ \<Rightarrow> _ \<Rightarrow> _ \<Rightarrow> bump_heuristics_init\<close> where
+  \<open>Bump_Heuristics_Init a b c d \<equiv> Tuple4 a b c d\<close>
+
+lemmas bump_heuristics_init_splits = Tuple4.tuple4.splits
+hide_fact tuple4.splits
+
+abbreviation get_stable_heuristics :: \<open>bump_heuristics_init \<Rightarrow> vmtf_remove_int_option_fst_As\<close> where
+  \<open>get_stable_heuristics \<equiv> Tuple4_a\<close>
+
+abbreviation get_focused_heuristics :: \<open>bump_heuristics_init \<Rightarrow> vmtf_remove_int_option_fst_As\<close> where
+  \<open>get_focused_heuristics \<equiv> Tuple4_b\<close>
+
+abbreviation is_focused_heuristics :: \<open>bump_heuristics_init \<Rightarrow> bool\<close> where
+  \<open>is_focused_heuristics \<equiv> Tuple4_c\<close>
+
+abbreviation is_stable_heuristics:: \<open>bump_heuristics_init \<Rightarrow> bool\<close> where
+  \<open>is_stable_heuristics x \<equiv> \<not>is_focused_heuristics x\<close>
+
+abbreviation get_bumped_variables :: \<open>bump_heuristics_init \<Rightarrow> nat list \<times> bool list\<close> where
+  \<open>get_bumped_variables \<equiv> Tuple4_d\<close>
+
+abbreviation set_stable_heuristics :: \<open>vmtf_remove_int_option_fst_As \<Rightarrow>bump_heuristics_init \<Rightarrow> _\<close> where
+  \<open>set_stable_heuristics \<equiv> Tuple4.set_a\<close>
+
+abbreviation set_focused_heuristics :: \<open>vmtf_remove_int_option_fst_As \<Rightarrow>bump_heuristics_init \<Rightarrow> _\<close> where
+  \<open>set_focused_heuristics \<equiv> Tuple4.set_b\<close>
+
+abbreviation set_is_focused_heuristics :: \<open>bool \<Rightarrow>bump_heuristics_init \<Rightarrow> _\<close> where
+  \<open>set_is_focused_heuristics \<equiv> Tuple4.set_c\<close>
+
+abbreviation set_bumped_variables :: \<open>nat list \<times> bool list \<Rightarrow>bump_heuristics_init \<Rightarrow> _\<close> where
+  \<open>set_bumped_variables \<equiv> Tuple4.set_d\<close>
+
+definition get_unit_trail where
+  \<open>get_unit_trail M = (rev (takeWhile (\<lambda>x. \<not>is_decided x) (rev M)))\<close>
+
+definition bump_heur_init :: \<open>_ \<Rightarrow> _ \<Rightarrow> bump_heuristics_init set\<close> where
+  \<open>bump_heur_init \<A> M = {x.
+      get_stable_heuristics x \<in> isa_vmtf_init \<A> M \<and>
+       get_focused_heuristics x \<in> isa_vmtf_init \<A> M \<and>
+  (get_bumped_variables x, set (fst (get_bumped_variables x))) \<in> distinct_atoms_rel \<A> \<and>
+  count_decided M = 0
+  }\<close>
+
+
+lemma get_unit_trail_count_decided_0[simp]: \<open>count_decided M = 0 \<Longrightarrow> get_unit_trail M = M\<close>
+  by (auto simp: get_unit_trail_def count_decided_0_iff)
+   (metis rev_swap set_rev takeWhile_eq_all_conv)
+
+
+subsection \<open>Access Function\<close>
+
+(*TODO: replace by proper shared init later*)
+definition vmtf_heur_import_variable :: \<open>nat \<Rightarrow> vmtf_remove_int_option_fst_As \<Rightarrow> _\<close> where
+  \<open>vmtf_heur_import_variable L = (\<lambda>(n, stmp, fst, last, cnext).
+     (vmtf_cons n L cnext stmp, stmp+1, fst, Some L, cnext))\<close>
+
+definition bump_heur_import_variable where
+  \<open>bump_heur_import_variable L x = (case x of Bump_Heuristics_Init hstable focused foc n \<Rightarrow>
+    Bump_Heuristics_Init (vmtf_heur_import_variable L hstable) (vmtf_heur_import_variable L focused) foc n)\<close>
+
+definition initialise_VMTF :: \<open>nat list \<Rightarrow> nat \<Rightarrow> vmtf_remove_int_option_fst_As nres\<close> where
+\<open>initialise_VMTF N n = do {
+   let A = replicate n (VMTF_Node 0 None None);
+   ASSERT(length N \<le> uint32_max);
+   (n, A, cnext) \<leftarrow> WHILE\<^sub>T
+      (\<lambda>(i, A, cnext). i < length_uint32_nat N)
+      (\<lambda>(i, A, cnext). do {
+        ASSERT(i < length_uint32_nat N);
+        let L = (N ! i);
+        ASSERT(L < length A);
+        ASSERT(cnext \<noteq> None \<longrightarrow> the cnext < length A);
+        ASSERT(i + 1 \<le> uint32_max);
+        RETURN (i + 1, vmtf_cons A L cnext (i), Some L)
+      })
+      (0, A, None);
+   RETURN ((A, n, cnext, (if N = [] then None else Some ((N!0))), cnext))
+  }\<close>
+
+definition (in -) distinct_atms_empty where
+  \<open>distinct_atms_empty _ = {}\<close>
+
+definition (in -) distinct_atms_int_empty where
+  \<open>distinct_atms_int_empty n = RETURN ([], replicate n False)\<close>
+
+
+lemma distinct_atms_int_empty_distinct_atms_empty:
+  \<open>(distinct_atms_int_empty, RETURN o distinct_atms_empty) \<in>
+     [\<lambda>n. (\<forall>L\<in>#\<L>\<^sub>a\<^sub>l\<^sub>l \<A>. atm_of L < n)]\<^sub>f nat_rel \<rightarrow> \<langle>distinct_atoms_rel \<A>\<rangle>nres_rel\<close>
+  apply (intro frefI nres_relI)
+  apply (auto simp: distinct_atoms_rel_alt_def distinct_atms_empty_def distinct_atms_int_empty_def)
+  by (metis atms_of_\<L>\<^sub>a\<^sub>l\<^sub>l_\<A>\<^sub>i\<^sub>n atms_of_def imageE)
+
+lemma initialise_VMTF:
+  shows  \<open>(uncurry initialise_VMTF, uncurry (\<lambda>N n. RES (isa_vmtf_init N []))) \<in>
+      [\<lambda>(N,n). (\<forall>L\<in># N. L < n) \<and> (distinct_mset N) \<and> size N < uint32_max \<and> set_mset N = set_mset \<A>]\<^sub>f
+      (\<langle>nat_rel\<rangle>list_rel_mset_rel) \<times>\<^sub>f nat_rel \<rightarrow> \<langle>Id\<rangle>nres_rel\<close>
+    (is \<open>(?init, ?R) \<in> _\<close>)
+proof -
+  have vmtf_ns_notin_empty: \<open>vmtf_ns_notin [] 0 (replicate n (VMTF_Node 0 None None))\<close> for n
+    unfolding vmtf_ns_notin_def
+    by auto
+
+  have K2: \<open>distinct N \<Longrightarrow> fst_As < length N \<Longrightarrow> N!fst_As \<in> set (take fst_As N) \<Longrightarrow> False\<close>
+    for fst_As x N
+    by (metis (no_types, lifting) in_set_conv_nth length_take less_not_refl min_less_iff_conj
+      nth_eq_iff_index_eq nth_take)
+  have W_ref: \<open>WHILE\<^sub>T (\<lambda>(i, A, cnext). i < length_uint32_nat N')
+        (\<lambda>(i, A, cnext). do {
+              _ \<leftarrow> ASSERT (i < length_uint32_nat N');
+              let L = (N' ! i);
+              _ \<leftarrow> ASSERT (L < length A);
+              _ \<leftarrow> ASSERT (cnext \<noteq> None \<longrightarrow> the cnext < length A);
+              _ \<leftarrow> ASSERT (i + 1 \<le> uint32_max);
+              RETURN
+               (i + 1,
+                vmtf_cons A L cnext (i), Some L)
+            })
+        (0, replicate n' (VMTF_Node 0 None None),
+         None)
+    \<le> SPEC(\<lambda>(i, A', cnext).
+      vmtf_ns (rev ((take i N'))) i A'
+        \<and> cnext = (option_last (take i N')) \<and>  i = length N' \<and>
+          length A' = n \<and> vmtf_ns_notin (rev ((take i N'))) i A'
+      )\<close>
+    (is \<open>_ \<le> SPEC ?P\<close>)
+    if H: \<open>case y of (N, n) \<Rightarrow>(\<forall>L\<in># N. L < n) \<and> distinct_mset N \<and> size N < uint32_max \<and>
+         set_mset N = set_mset \<A>\<close> and
+       ref: \<open>(x, y) \<in> \<langle>Id\<rangle>list_rel_mset_rel \<times>\<^sub>f nat_rel\<close> and
+       st[simp]: \<open>x = (N', n')\<close> \<open>y = (N, n)\<close>
+     for N N' n n' A x y
+  proof -
+  have [simp]: \<open>n = n'\<close> and NN': \<open>(N', N) \<in> \<langle>Id\<rangle>list_rel_mset_rel\<close>
+    using ref unfolding st by auto
+  then have dist: \<open>distinct N'\<close>
+    using NN' H by (auto simp: list_rel_def br_def list_mset_rel_def list.rel_eq
+      list_all2_op_eq_map_right_iff' distinct_image_mset_inj list_rel_mset_rel_def)
+
+  have L_N: \<open>\<forall>L\<in>set N'. L < n\<close>
+    using H ref by (auto simp: list_rel_def br_def list_mset_rel_def
+      list_all2_op_eq_map_right_iff' list_rel_mset_rel_def list.rel_eq)
+  let ?Q = \<open>\<lambda>(i, A', cnext).
+      vmtf_ns (rev ((take i N'))) i A' \<and> i \<le> length N' \<and>
+      cnext = (option_last (take i N')) \<and>
+      length A' = n \<and> vmtf_ns_notin (rev ((take i N'))) i A'\<close>
+  show ?thesis
+    apply (refine_vcg WHILET_rule[where R = \<open>measure (\<lambda>(i, _). length N' + 1 - i)\<close> and I = \<open>?Q\<close>])
+    subgoal by auto
+    subgoal by (auto intro: vmtf_ns.intros)
+    subgoal by auto
+    subgoal by auto
+    subgoal by auto
+    subgoal for S N' x2 A'
+      unfolding assert_bind_spec_conv vmtf_ns_notin_def
+      using L_N dist
+      by (auto 5 5 simp: take_Suc_conv_app_nth hd_drop_conv_nth nat_shiftr_div2
+          option_last_def hd_rev last_map intro!: vmtf_cons dest: K2)
+    subgoal by auto
+    subgoal
+      using L_N dist
+      by (auto simp: take_Suc_conv_app_nth hd_drop_conv_nth nat_shiftr_div2
+          option_last_def hd_rev last_map)
+    subgoal
+      using L_N dist
+      by (auto simp: last_take_nth_conv option_last_def)
+    subgoal
+      using H dist ref
+      by (auto simp: last_take_nth_conv option_last_def list_rel_mset_rel_imp_same_length)
+    subgoal
+      using L_N dist
+      by (auto 5 5 simp: take_Suc_conv_app_nth option_last_def hd_rev last_map intro!: vmtf_cons
+          dest: K2)
+    subgoal by (auto simp: take_Suc_conv_app_nth)
+    subgoal by (auto simp: take_Suc_conv_app_nth)
+    subgoal by auto
+    subgoal
+      using L_N dist
+      by (auto 5 5 simp: take_Suc_conv_app_nth hd_rev last_map option_last_def
+          intro!: vmtf_notin_vmtf_cons dest: K2 split: if_splits)
+    subgoal by auto
+    subgoal by auto
+    subgoal by auto
+    subgoal by auto
+    subgoal by auto
+    subgoal by auto
+    done
+  qed
+  have [simp]: \<open>vmtf_\<L>\<^sub>a\<^sub>l\<^sub>l n' [] ((set N, {}))\<close>
+    if \<open>(N, n') \<in> \<langle>Id\<rangle>list_rel_mset_rel\<close> for N N' n'
+    using that unfolding vmtf_\<L>\<^sub>a\<^sub>l\<^sub>l_def
+    by (auto simp: \<L>\<^sub>a\<^sub>l\<^sub>l_def atms_of_def image_image image_Un list_rel_def
+       br_def list_mset_rel_def list_all2_op_eq_map_right_iff'
+      list_rel_mset_rel_def list.rel_eq)
+  have in_N_in_N1: \<open>L \<in> set N' \<Longrightarrow>  L \<in> atms_of (\<L>\<^sub>a\<^sub>l\<^sub>l N)\<close>
+    if  \<open>(N', N) \<in> list_mset_rel\<close> for L N N' y
+    using that by (auto simp: \<L>\<^sub>a\<^sub>l\<^sub>l_def atms_of_def image_image image_Un list_rel_def
+      list.rel_eq br_def list_mset_rel_def list_all2_op_eq_map_right_iff')
+
+  have length_ba: \<open>\<forall>L\<in># N. L < length ba \<Longrightarrow> L \<in> atms_of (\<L>\<^sub>a\<^sub>l\<^sub>l N) \<Longrightarrow>
+     L < length ba\<close>
+    if \<open>(N', y) \<in> \<langle>Id\<rangle>list_rel_mset_rel\<close>
+    for L ba N N' y
+    using that
+    by (auto simp: \<L>\<^sub>a\<^sub>l\<^sub>l_def nat_shiftr_div2 list.rel_eq
+      atms_of_def image_image image_Un split: if_splits)
+  show ?thesis
+    supply list.rel_eq[simp]
+    apply (intro frefI nres_relI)
+    unfolding initialise_VMTF_def uncurry_def conc_Id id_def isa_vmtf_init_def
+      distinct_atms_int_empty_def nres_monad1
+    apply (subst Let_def)
+    apply (refine_vcg)
+    subgoal by (auto dest: list_rel_mset_rel_imp_same_length)
+      apply (rule W_ref[THEN order_trans]; assumption?)
+    subgoal for N' N'n' n' Nn
+      apply (auto dest: list_rel_mset_rel_imp_same_length simp: vmtf_def)
+      apply (rule exI[of _ \<open>(rev (fst N'))\<close>])
+      apply (rule_tac exI[of _ \<open>[]\<close>])
+      apply (auto dest: list_rel_mset_rel_imp_same_length simp: vmtf_def hd_rev last_conv_nth rev_nth
+        atms_of_\<L>\<^sub>a\<^sub>l\<^sub>l_\<A>\<^sub>i\<^sub>n)
+      apply (auto dest: list_rel_mset_rel_imp_same_length simp: vmtf_def hd_rev last_conv_nth rev_nth
+        atms_of_\<L>\<^sub>a\<^sub>l\<^sub>l_\<A>\<^sub>i\<^sub>n list_rel_mset_rel_def list_mset_rel_def br_def)
+      done
+    done
+qed
+
+definition initialize_Bump_Init :: \<open>nat list \<Rightarrow> nat \<Rightarrow> bump_heuristics_init nres\<close> where
+  \<open>initialize_Bump_Init A n = do {
+  focused \<leftarrow> initialise_VMTF A n;
+  hstable \<leftarrow> initialise_VMTF A n;
+  to_remove \<leftarrow> distinct_atms_int_empty n;
+  RETURN (Tuple4 hstable focused False to_remove)
+  }\<close>
+
+lemma specify_left_RES:
+  assumes "m \<le> RES \<Phi>"
+  assumes "\<And>x. x \<in> \<Phi> \<Longrightarrow> f x \<le> M"  
+  shows "do { x \<leftarrow> m; f x } \<le> M"
+  using assms by (auto simp: pw_le_iff refine_pw_simps)
+
+lemma initialize_Bump_Init:
+  shows  \<open>(uncurry initialize_Bump_Init, uncurry (\<lambda>N n. RES (bump_heur_init N []))) \<in>
+      [\<lambda>(N,n). (\<forall>L\<in># N. L < n) \<and> (distinct_mset N) \<and> size N < uint32_max \<and> set_mset N = set_mset \<A>]\<^sub>f
+      (\<langle>nat_rel\<rangle>list_rel_mset_rel) \<times>\<^sub>f nat_rel \<rightarrow> \<langle>Id\<rangle>nres_rel\<close>
+    (is \<open>(?init, ?R) \<in> _\<close>)
+  unfolding initialize_Bump_Init_def uncurry_def distinct_atms_int_empty_def nres_monad1
+  apply (intro frefI nres_relI)
+  apply (refine_rcg)
+  apply hypsubst
+  apply (rule specify_left_RES[OF initialise_VMTF[where \<A>=\<A>, THEN fref_to_Down_curry, unfolded conc_fun_RES]])
+  apply assumption+
+  apply (rule specify_left_RES[OF initialise_VMTF[where \<A>=\<A>, THEN fref_to_Down_curry, unfolded conc_fun_RES]])
+  apply assumption+
+  apply (auto simp: bump_heur_init_def distinct_atoms_rel_def distinct_hash_atoms_rel_def
+    atoms_hash_rel_def intro!: relcompI)
+  done
+
+
+type_synonym bump_heuristics_option_fst_As = \<open>vmtf_remove_int_option_fst_As\<close>
+
+lemma isa_vmtf_init_consD:
+  \<open>((ns, m, fst_As, lst_As, next_search)) \<in> isa_vmtf_init \<A> M \<Longrightarrow>
+     ((ns, m, fst_As, lst_As, next_search)) \<in> isa_vmtf_init \<A> (L # M)\<close>
+  by (auto simp: isa_vmtf_init_def dest: vmtf_consD)
+
+lemma isa_vmtf_init_consD':
+  \<open>vm \<in> isa_vmtf_init \<A> M \<Longrightarrow> vm \<in> isa_vmtf_init \<A> (L # M)\<close>
+  by (auto simp: isa_vmtf_init_def dest: vmtf_consD)
+
+(*TODO share*)
+
+lemma vmtf_cong:
+  \<open>set_mset \<A> = set_mset \<B> \<Longrightarrow> L \<in> vmtf \<A> M \<Longrightarrow> L \<in> vmtf \<B> M\<close>
+  using \<L>\<^sub>a\<^sub>l\<^sub>l_cong[of \<A> \<B>] atms_of_\<L>\<^sub>a\<^sub>l\<^sub>l_cong[of \<A> \<B>]
+  unfolding vmtf_def vmtf_\<L>\<^sub>a\<^sub>l\<^sub>l_def
+  by auto
+lemma isa_vmtf_init_cong:
+  \<open>set_mset \<A> = set_mset \<B> \<Longrightarrow> L \<in> isa_vmtf_init \<A> M \<Longrightarrow> L \<in> isa_vmtf_init \<B> M\<close>
+  using \<L>\<^sub>a\<^sub>l\<^sub>l_cong[of \<A> \<B>] atms_of_\<L>\<^sub>a\<^sub>l\<^sub>l_cong[of \<A> \<B>] vmtf_cong[of \<A> \<B>]
+  unfolding isa_vmtf_init_def vmtf_\<L>\<^sub>a\<^sub>l\<^sub>l_def
+  by auto
+
+
+lemma bump_heur_init_consD':
+  \<open>vm \<in> bump_heur_init \<A> M \<Longrightarrow> vm \<in> bump_heur_init \<A> (Propagated L n # M)\<close>
+  by (auto simp: bump_heur_init_def dest: isa_vmtf_init_consD')
+
+end
